src/case_study/program_logic/lifting.v
@@ -7,7 +7,7 @@ From iris.prelude Require Import options.
 
 Section lifting.
 Context `{!irisGS_gen hlc Λ Σ}.
-Implicit Types s : stuckness.
+Implicit Types s : (stuckness * A).
 Implicit Types v : val Λ.
 Implicit Types e : expr Λ.
 Implicit Types σ : state Λ.
@@ -18,24 +18,24 @@ Local Hint Resolve reducible_no_obs_reducible : core.
 
 Lemma wp_lift_step_fupdN s E Φ e1 :
   to_val e1 = None →
-  (∀ σ1 ns κ κs nt, (⚡={next_state σ1}=> |==> state_interp σ1 ns (κ ++ κs) nt) ={E,∅}=∗
-    ⌜if s is NotStuck then reducible e1 σ1 else True⌝ ∗
+  (∀ σ1 ns κ κs nt, (state_interp σ1 ns (κ ++ κs) nt) ={E,∅}=∗
+    ⌜if s.1 is NotStuck then reducible e1 σ1 else True⌝ ∗
     ∀ e2 σ2 efs, ⌜prim_step e1 σ1 κ e2 σ2 efs⌝ -∗
       £ (S $ num_laters_per_step ns)
       ={∅}▷=∗^(S $ num_laters_per_step ns) |={∅,E}=>
-      (⚡={next_state σ2}=> |==> state_interp σ2 (S ns) κs (length efs + nt)) ∗
-      WP e2 @ s; E {{ Φ }} ∗
+      state_interp σ2 (S ns) κs (length efs + nt) ∗
+      (⚡={next_state (next_a e1 s.2)}=> WP e2 @ s; E {{ Φ }}) ∗
       [∗ list] ef ∈ efs, WP ef @ s; ⊤ {{ fork_post }})
   ⊢ WP e1 @ s; E {{ Φ }}.
 Proof. by rewrite wp_unfold /wp_pre=>->. Qed.
 
 Lemma wp_lift_step_fupd s E Φ e1 :
   to_val e1 = None →
-  (∀ σ1 ns κ κs nt, (⚡={next_state σ1}=> |==> state_interp σ1 ns (κ ++ κs) nt) ={E,∅}=∗
-    ⌜if s is NotStuck then reducible e1 σ1 else True⌝ ∗
+  (∀ σ1 ns κ κs nt, (state_interp σ1 ns (κ ++ κs) nt) ={E,∅}=∗
+    ⌜if s.1 is NotStuck then reducible e1 σ1 else True⌝ ∗
     ∀ e2 σ2 efs, ⌜prim_step e1 σ1 κ e2 σ2 efs⌝ -∗ £ 1 ={∅}=∗ ▷ |={∅,E}=>
-      (⚡={next_state σ2}=> |==> state_interp σ2 (S ns) κs (length efs + nt)) ∗
-      WP e2 @ s; E {{ Φ }} ∗
+      (state_interp σ2 (S ns) κs (length efs + nt)) ∗
+      (⚡={next_state (next_a e1 s.2)}=> WP e2 @ s; E {{ Φ }}) ∗
       [∗ list] ef ∈ efs, WP ef @ s; ⊤ {{ fork_post }})
   ⊢ WP e1 @ s; E {{ Φ }}.
 Proof.
@@ -48,24 +48,24 @@ Proof.
   iApply step_fupd_intro; done.
 Qed.
 
-Lemma wp_lift_stuck E Φ e :
-  to_val e = None →
-  (∀ σ ns κs nt, (⚡={next_state σ}=> |==> state_interp σ ns κs nt) ={E,∅}=∗ ⌜stuck e σ⌝)
-  ⊢ WP e @ E ?{{ Φ }}.
-Proof.
-  rewrite wp_unfold /wp_pre=>->. iIntros "H" (σ1 ns κ κs nt) "Hσ".
-  iMod ("H" with "Hσ") as %[? Hirr]. iModIntro. iSplit; first done.
-  iIntros (e2 σ2 efs ?). by case: (Hirr κ e2 σ2 efs).
-Qed.
+(* Lemma wp_lift_stuck E Φ e : *)
+(*   to_val e = None → *)
+(*   (∀ σ ns κs nt, (state_interp σ ns κs nt) ={E,∅}=∗ ⌜stuck e σ⌝) *)
+(*   ⊢ WP e @ E ?{{ Φ }}. *)
+(* Proof. *)
+(*   rewrite wp_unfold /wp_pre=>->. iIntros "H" (σ1 ns κ κs nt) "Hσ". *)
+(*   iMod ("H" with "Hσ") as %[? Hirr]. iModIntro. iSplit; first done. *)
+(*   iIntros (e2 σ2 efs ?). by case: (Hirr κ e2 σ2 efs). *)
+(* Qed. *)
 
 (** Derived lifting lemmas. *)
 Lemma wp_lift_step s E Φ e1 :
   to_val e1 = None →
-  (∀ σ1 ns κ κs nt, (⚡={next_state σ1}=> |==> state_interp σ1 ns (κ ++ κs) nt) ={E,∅}=∗
-    ⌜if s is NotStuck then reducible e1 σ1 else True⌝ ∗
+  (∀ σ1 ns κ κs nt, (state_interp σ1 ns (κ ++ κs) nt) ={E,∅}=∗
+    ⌜if s.1 is NotStuck then reducible e1 σ1 else True⌝ ∗
     ▷ ∀ e2 σ2 efs, ⌜prim_step e1 σ1 κ e2 σ2 efs⌝ -∗ £ 1 ={∅,E}=∗
-      (⚡={next_state σ2}=> |==> state_interp σ2 (S ns) κs (length efs + nt)) ∗
-      WP e2 @ s; E {{ Φ }} ∗
+      (state_interp σ2 (S ns) κs (length efs + nt)) ∗
+      (⚡={next_state (next_a e1 s.2)}=> WP e2 @ s; E {{ Φ }}) ∗
       [∗ list] ef ∈ efs, WP ef @ s; ⊤ {{ fork_post }})
   ⊢ WP e1 @ s; E {{ Φ }}.
 Proof.
@@ -74,43 +74,43 @@ Proof.
 Qed.
 
 Lemma wp_lift_pure_step_no_fork `{!Inhabited (state Λ)} s E E' Φ e1 :
-  (∀ σ1, if s is NotStuck then reducible e1 σ1 else to_val e1 = None) →
+  (∀ σ1, if s.1 is NotStuck then reducible e1 σ1 else to_val e1 = None) →
   (∀ κ σ1 e2 σ2 efs, prim_step e1 σ1 κ e2 σ2 efs → κ = [] ∧ σ2 = σ1 ∧ efs = []) →
-  (|={E}[E']▷=> ∀ κ e2 efs σ, ⌜prim_step e1 σ κ e2 σ efs⌝ -∗ £ 1 -∗ WP e2 @ s; E {{ Φ }})
+  (|={E}[E']▷=> ∀ κ e2 efs σ, ⌜prim_step e1 σ κ e2 σ efs⌝ -∗ £ 1 -∗ ⚡={next_state (next_a e1 s.2)}=> WP e2 @ s; E {{ Φ }})
   ⊢ WP e1 @ s; E {{ Φ }}.
 Proof.
   iIntros (Hsafe Hstep) "H". iApply wp_lift_step.
-  { specialize (Hsafe inhabitant). destruct s; eauto using reducible_not_val. }
+  { specialize (Hsafe inhabitant). destruct s as [s a];simpl in *;destruct s; eauto using reducible_not_val. }
   iIntros (σ1 ns κ κs nt) "Hσ". iMod "H".
   iApply fupd_mask_intro; first set_solver. iIntros "Hclose". iSplit.
-  { iPureIntro. destruct s; done. }
+  { iPureIntro. destruct s as [s a];simpl in *;destruct s; done. }
   iNext. iIntros (e2 σ2 efs ?) "Hcred".
   destruct (Hstep κ σ1 e2 σ2 efs) as (-> & <- & ->); auto.
   iMod "Hclose" as "_". iMod "H". iModIntro.
   iDestruct ("H" with "[//] Hcred") as "$".
-  iSplitL =>//. iModIntro. iMod "Hσ". iModIntro.
+  iSplitL =>//.
   by iApply state_interp_mono.
 Qed.
 
-Lemma wp_lift_pure_stuck `{!Inhabited (state Λ)} E Φ e :
-  (∀ σ, stuck e σ) →
-  True ⊢ WP e @ E ?{{ Φ }}.
-Proof.
-  iIntros (Hstuck) "_". iApply wp_lift_stuck.
-  - destruct(to_val e) as [v|] eqn:He; last done.
-    rewrite -He. by case: (Hstuck inhabitant).
-  - iIntros (σ ns κs nt) "_". iApply fupd_mask_intro; auto with set_solver.
-Qed.
+(* Lemma wp_lift_pure_stuck `{!Inhabited (state Λ)} E Φ e : *)
+(*   (∀ σ, stuck e σ) → *)
+(*   True ⊢ WP e @ E ?{{ Φ }}. *)
+(* Proof. *)
+(*   iIntros (Hstuck) "_". iApply wp_lift_stuck. *)
+(*   - destruct(to_val e) as [v|] eqn:He; last done. *)
+(*     rewrite -He. by case: (Hstuck inhabitant). *)
+(*   - iIntros (σ ns κs nt) "_". iApply fupd_mask_intro; auto with set_solver. *)
+(* Qed. *)
 
 (* Atomic steps don't need any mask-changing business here, one can
    use the generic lemmas here. *)
 Lemma wp_lift_atomic_step_fupd {s E1 E2 Φ} e1 :
   to_val e1 = None →
-  (∀ σ1 ns κ κs nt, (⚡={next_state σ1}=> |==> state_interp σ1 ns (κ ++ κs) nt) ={E1}=∗
-    ⌜if s is NotStuck then reducible e1 σ1 else True⌝ ∗
+  (∀ σ1 ns κ κs nt, (state_interp σ1 ns (κ ++ κs) nt) ={E1}=∗
+    ⌜if s.1 is NotStuck then reducible e1 σ1 else True⌝ ∗
     ∀ e2 σ2 efs, ⌜prim_step e1 σ1 κ e2 σ2 efs⌝ -∗ £ 1 ={E1}[E2]▷=∗
-      (⚡={next_state σ2}=> |==> state_interp σ2 (S ns) κs (length efs + nt)) ∗
-      from_option Φ False (to_val e2) ∗
+      (state_interp σ2 (S ns) κs (length efs + nt)) ∗
+      from_option (λ v, ⚡={next_state (next_a e1 s.2)}=> Φ v) False (to_val e2) ∗
       [∗ list] ef ∈ efs, WP ef @ s; ⊤ {{ fork_post }})
   ⊢ WP e1 @ s; E1 {{ Φ }}.
 Proof.
@@ -123,16 +123,16 @@ Proof.
   iApply fupd_mask_intro; first set_solver. iIntros "Hclose !>".
   iMod "Hclose" as "_". iMod "H" as "($ & HQ & $)".
   destruct (to_val e2) eqn:?; last by iExFalso.
-  iApply wp_value; last done. by apply of_to_val.
+  simpl. iModIntro. iModIntro. iApply wp_value; last done. by apply of_to_val.
 Qed.
 
 Lemma wp_lift_atomic_step {s E Φ} e1 :
   to_val e1 = None →
-  (∀ σ1 ns κ κs nt, (⚡={next_state σ1}=> |==> state_interp σ1 ns (κ ++ κs) nt) ={E}=∗
-    ⌜if s is NotStuck then reducible e1 σ1 else True⌝ ∗
+  (∀ σ1 ns κ κs nt, (state_interp σ1 ns (κ ++ κs) nt) ={E}=∗
+    ⌜if s.1 is NotStuck then reducible e1 σ1 else True⌝ ∗
     ▷ ∀ e2 σ2 efs, ⌜prim_step e1 σ1 κ e2 σ2 efs⌝ -∗ £ 1 ={E}=∗
-      (⚡={next_state σ2}=> |==> state_interp σ2 (S ns) κs (length efs + nt)) ∗
-      from_option Φ False (to_val e2) ∗
+      (state_interp σ2 (S ns) κs (length efs + nt)) ∗
+      from_option (λ v, ⚡={next_state (next_a e1 s.2)}=> Φ v) False (to_val e2) ∗
       [∗ list] ef ∈ efs, WP ef @ s; ⊤ {{ fork_post }})
   ⊢ WP e1 @ s; E {{ Φ }}.
 Proof.
@@ -143,10 +143,10 @@ Proof.
 Qed.
 
 Lemma wp_lift_pure_det_step_no_fork `{!Inhabited (state Λ)} {s E E' Φ} e1 e2 :
-  (∀ σ1, if s is NotStuck then reducible e1 σ1 else to_val e1 = None) →
+  (∀ σ1, if s.1 is NotStuck then reducible e1 σ1 else to_val e1 = None) →
   (∀ σ1 κ e2' σ2 efs', prim_step e1 σ1 κ e2' σ2 efs' →
     κ = [] ∧ σ2 = σ1 ∧ e2' = e2 ∧ efs' = []) →
-  (|={E}[E']▷=> £ 1 -∗ WP e2 @ s; E {{ Φ }}) ⊢ WP e1 @ s; E {{ Φ }}.
+  (|={E}[E']▷=> £ 1 -∗ (⚡={next_state (next_a e1 s.2)}=> WP e2 @ s; E {{ Φ }})) ⊢ WP e1 @ s; E {{ Φ }}.
 Proof.
   iIntros (? Hpuredet) "H". iApply (wp_lift_pure_step_no_fork s E E'); try done.
   { naive_solver. }
@@ -154,31 +154,44 @@ Proof.
   iIntros (κ e' efs' σ (_&?&->&?)%Hpuredet); auto.
 Qed.
 
-Lemma wp_pure_step_fupd `{!Inhabited (state Λ)} s E E' e1 e2 φ n Φ :
-  PureExec φ n e1 e2 →
-  φ →
-  (|={E}[E']▷=>^n £ n -∗ WP e2 @ s; E {{ Φ }}) ⊢ WP e1 @ s; E {{ Φ }}.
-Proof.
-  iIntros (Hexec Hφ) "Hwp". specialize (Hexec Hφ).
-  iInduction Hexec as [e|n e1 e2 e3 [Hsafe ?]] "IH"; simpl.
-  { iMod lc_zero as "Hz". by iApply "Hwp". }
-  iApply wp_lift_pure_det_step_no_fork.
-  - intros σ. specialize (Hsafe σ). destruct s; eauto using reducible_not_val.
-  - done.
-  - iApply (step_fupd_wand with "Hwp").
-    iIntros "Hwp Hone". iApply "IH".
-    iApply (step_fupdN_wand with "Hwp").
-    iIntros "Hwp Hc". iApply ("Hwp" with "[Hone Hc]").
-    rewrite (lc_succ n). iFrame.
-Qed.
+Fixpoint n_next_state (n : nat) (a : A) (P : iProp Σ) :=
+  match n with
+  | 0 => P
+  | S n => (⚡={next_state a}=> (n_next_state n a P))%I
+  end.
 
-Lemma wp_pure_step_later `{!Inhabited (state Λ)} s E e1 e2 φ n Φ :
-  PureExec φ n e1 e2 →
-  φ →
-  ▷^n (£ n -∗ WP e2 @ s; E {{ Φ }}) ⊢ WP e1 @ s; E {{ Φ }}.
-Proof.
-  intros Hexec ?. rewrite -wp_pure_step_fupd //. clear Hexec.
-  enough (∀ P, ▷^n P ⊢ |={E}▷=>^n P) as Hwp by apply Hwp. intros ?.
-  induction n as [|n IH]; by rewrite //= -step_fupd_intro // IH.
-Qed.
+(* Lemma wp_pure_step_fupd `{!Inhabited (state Λ)} s E E' e1 e2 φ n Φ : *)
+(*   PureExec φ n e1 e2 → *)
+(*   φ → *)
+(*   (|={E}[E']▷=>^n £ n -∗ n_next_state n (next_a e1 s.2) (WP e2 @ s; E {{ Φ }}) *)
+(*   (* match n with *) *)
+(*   (* | 0 => WP e2 @ s; E {{ Φ }} *) *)
+(*   (* | _ => ⚡={next_state (next_a e1 s.2)}=> WP e2 @ s; E {{ Φ }}   *) *)
+(*   (*  end *)) *)
+(*     ⊢ WP e1 @ s; E {{ Φ }}. *)
+(* Proof. *)
+(*   iIntros (Hexec Hφ) "Hwp". specialize (Hexec Hφ). *)
+(*   iInduction Hexec as [e|n e1 e2 e3 [Hsafe ?]] "IH"; simpl. *)
+(*   { iMod lc_zero as "Hz". by iApply "Hwp". } *)
+(*   iApply wp_lift_pure_det_step_no_fork. *)
+(*   - intros σ. specialize (Hsafe σ). destruct s as [s a];simpl in *;destruct s; eauto using reducible_not_val. *)
+(*   - done. *)
+(*   - iApply (step_fupd_wand with "Hwp"). *)
+(*     iIntros "Hwp Hone". *)
+(*     iDestruct ("IH" with "[Hwp]") as "HH". *)
+(*     { } *)
+(*     iApply (step_fupdN_wand with "Hwp"). *)
+(*     iIntros "Hwp Hc". iApply ("Hwp" with "[Hone Hc]"). *)
+(*     rewrite (lc_succ n). iFrame. *)
+(* Qed. *)
+
+(* Lemma wp_pure_step_later `{!Inhabited (state Λ)} s E e1 e2 φ n Φ : *)
+(*   PureExec φ n e1 e2 → *)
+(*   φ → *)
+(*   ▷^n (£ n -∗ WP e2 @ s; E {{ Φ }}) ⊢ WP e1 @ s; E {{ Φ }}. *)
+(* Proof. *)
+(*   intros Hexec ?. rewrite -wp_pure_step_fupd //. clear Hexec. *)
+(*   enough (∀ P, ▷^n P ⊢ |={E}▷=>^n P) as Hwp by apply Hwp. intros ?. *)
+(*   induction n as [|n IH]; by rewrite //= -step_fupd_intro // IH. *)
+(* Qed. *)
 End lifting.
